updates

Veritas.Interleave.fsti
@@ -3,6 +3,24 @@ module Veritas.Interleave
 open FStar.Seq
 open Veritas.SeqAux
 
+(* sequence of sequences *)
+type sseq (a:Type) = seq (seq a)
+
+(* sum of lengths of all sequences in a sequence of seqs *)
+val flat_length (#a:Type) (ss: sseq a): Tot nat
+
+(* flat length of an empty sseq *)
+val lemma_flat_length_empty (#a:Type):
+  Lemma (flat_length (empty #(seq a)) = 0)
+
+(* appending a singleton adds to the flat length *)
+val lemma_flat_length_app1 (#a:Type) (ss: sseq a) (s: seq a):
+  Lemma (flat_length ss + length s = flat_length (append1 ss s))
+
+(* appending adds to the flat length *)
+val lemma_flat_length_app (#a:Type) (ss1 ss2: sseq a):
+  Lemma (flat_length ss1 + flat_length ss2 = flat_length (append ss1 ss2))
+
 (* interleaving of n sequences *)
 val interleave (#a:eqtype): seq a -> ss:(seq (seq a)) -> Type 
 
@@ -19,6 +37,23 @@ val interleave_map_inv (#a:eqtype) (s: seq a) (ss: seq (seq a))
       (prf:interleave #a s ss) (i: seq_index ss) (j: seq_index (index ss i)): 
   Tot (k: seq_index s{index s k = index (index ss i) j})
 
+(* length of an interleaving is the sum of the lengths of the individual sequences *)
+val lemma_interleave_length (#a:eqtype) (s: seq a) (ss: seq (seq a){interleave s ss}):
+  Lemma (length s = flat_length ss)
+
+(* an interleave constructor that specifies the construction of 
+ * an interleaving *)
+type interleave_ctor (#a:eqtype) (ss: seq (seq a)) =
+  (i: seq_index ss) -> (j: seq_index (index ss i)) -> k:nat{k < flat_length ss}
+
+(* from an interleave_ constructor we can get an interleaving *)
+val interleaved_seq (#a:eqtype) (ss: seq (seq a)) (ic: interleave_ctor ss):
+  Tot (s: seq a{interleave s ss})
+
+(* we can also construct a proof of interleaving *)
+val interleaving_prf (#a: eqtype) (ss: seq (seq a)) (ic: interleave_ctor ss):
+  Tot (interleave (interleaved_seq ss ic) ss)
+
 (* sortedness of a sequence *)
 type sorted (#a:Type) (lte: a -> a -> bool) (s: seq a) = 
   forall (i:seq_index s). i > 0 ==> index s (i - 1) `lte` index s i
@@ -26,5 +61,11 @@ type sorted (#a:Type) (lte: a -> a -> bool) (s: seq a) =
 (* sort-merge interleaving *)
 val sort_merge (#a:eqtype) (lte: a-> a-> bool) 
                (ss: seq (seq a){forall (i:seq_index ss). sorted lte (index ss i)}): 
-  s:(seq a){interleave s ss /\ sorted lte s} 
-    
+  Tot (interleave_ctor ss)
+
+val lemma_sort_merge (#a:eqtype) (lte: a -> a -> bool)
+  (ss: seq (seq a){forall (i: seq_index ss). sorted lte (index ss i)}):
+  Lemma (requires (True))
+        (ensures (sorted lte (interleaved_seq ss (sort_merge lte ss))))
+        [SMTPat (sort_merge lte ss)]
+
